secure_api/box/experimental_box/Box.PKAE.fst
@@ -12,24 +12,61 @@ open Box.Plain
 module AE = Box.AE
 module ODH = Box.ODH
 module MM = FStar.Monotonic.Map
-module SPEC = Spec.SecretBox
+module AE_Spec = Spec.SecretBox
+module ODH_Spec = Spec.Curve25519
+module H = Spec.HSalsa20
 
-let id = ODH.id
 assume val random_bytes: n:(n:nat{n<=32}) -> unit -> lbytes n
 
+assume val pkae_flag: bool
+
+#set-options "--z3rlimit 300 --max_ifuel 1 --max_fuel 1"
+// For some reason it doesn't verify if there is an additional refinement on the output of secretbox_open_easy
 let secretbox_scheme =
-  AE.ES (random_bytes 32) SPEC.secretbox_easy SPEC.secretbox_open_easy
+  AE.ES #(AE_Spec.keylen) #(AE_Spec.noncelen) (fun n -> n / Spec.Salsa20.blocklen < pow2 32) (fun n -> n >= 16 && (n - 16) / Spec.Salsa20.blocklen < pow2 32) (random_bytes 32) AE_Spec.secretbox_easy AE_Spec.secretbox_open_easy
 
-let ae_package_log_key = i:id
-let ae_package_log_value (i:id)  = ae_package
-let ae_package_log_range (#id:eqtype) (i:id) (pp:plain_package) (nonce_length:(n:nat{n<=32})) (k:message_log_key nonce_length) = message_log_value i pp
-let ae_package_log_inv (#pp:plain_package) (#nonce_length:(n:nat{n<=32})) (#id:eqtype) (i:id) (f:MM.map' (message_log_key nonce_length) (message_log_range i pp nonce_length)) = True
+let ae_params = AE.GP AE_Spec.keylen AE_Spec.noncelen secretbox_scheme
 
-let message_log (#pp:plain_package) (#id:eqtype) (rgn:erid) (nonce_length:(n:nat{n<=32})) (i:id) =
-  MM.t rgn (message_log_key nonce_length) (message_log_range i pp nonce_length) (message_log_inv i)
+let pp = PP (AE.get_ae_flagGT ae_params) (fun n -> n / Spec.Salsa20.blocklen < pow2 32)
 
-//noeq abstract type pkae_package =
-//  | PKAE_P :
+let kp = AE.create_ae_key_package ODH.id AE_Spec.keylen
 
+let ae_package_log_key = i:ODH.id
+let ae_package_log_value (i:ODH.id) = (ap:AE.ae_package #ODH.id #i #AE_Spec.keylen kp ae_params pp)
+let ae_package_log_range (k:ae_package_log_key) = ae_package_log_value k
+let ae_package_log_inv (f:MM.map' (ae_package_log_key) (ae_package_log_range))  = True
 
-let gen = ODH.gen_dh
+let ae_package_log (rgn:erid) =
+  MM.t rgn (ae_package_log_key) (ae_package_log_range) (ae_package_log_inv)
+
+let zero_nonce = Seq.create H.noncelen (UInt8.uint_to_t 0)
+let hsalsa20_hash input = H.hsalsa20 input zero_nonce
+
+let odh_params = ODH.OP (ODH_Spec.serialized_point_length) (ODH_Spec.scalar_length) (H.keylen) (ODH_Spec.base_point) (ODH_Spec.scalarmult) (hsalsa20_hash)
+
+noeq abstract type pkae_package =
+  | PKAE_P :
+    op_rgn:erid ->
+    op: ODH.odh_package #AE_Spec.keylen #(AE.key AE_Spec.keylen #ODH.id) kp odh_params ->
+    ap_log_rgn:erid ->
+    ap_log: ae_package_log ap_log_rgn ->
+    pkae_package
+
+val create_pkae_package: rgn:erid -> ST pkae_package
+  (requires (fun h0 -> True))
+  (ensures (fun h0 pkae_p h1 ->
+    modifies (Set.singleton rgn) h0 h1
+  ))
+let create_pkae_package rgn =
+  let pkae_rgn = new_region rgn in
+  let odh_rgn = new_region pkae_rgn in
+  let ap_log_rgn = new_region pkae_rgn in
+  let op = ODH.create_odh_package kp odh_params odh_rgn in
+  let ap_log = MM.alloc #ap_log_rgn #ae_package_log_key #ae_package_log_range #ae_package_log_inv in
+  PKAE_P odh_rgn op ap_log_rgn ap_log
+
+let gen = ODH.gen_dh odh_params
+
+val encrypt: #id:eqtype -> #i:id -> #key_length:(n:nat{n<=32}) -> #kp:KEY.key_package #id key_length (key key_length #id) -> #aparams:ae_parameters{key_length = aparams.keylength} -> #pp:plain_package{ valid_ae_plain_package aparams pp} ->  ap:ae_package #id #i #key_length kp aparams pp -> k:key key_length i -> n:nonce aparams.nonce_length -> p:protected_plain pp i -> ST ciphertext
+
+let encrypt = ODH.odh_package
