secure_api/box/experimental_box/Box.Plain.fst
@@ -4,26 +4,23 @@ module KEY = Box.Key
 
 open FStar.Endianness
 
-abstract type plain_package =
+noeq type plain_package =
   | PP:
-    b:bool ->
+    flag:Type0 ->
+    valid_length:(nat -> bool) ->
     plain_package
 
-val get_flag: pp:plain_package -> GTot bool
-let get_flag pp = pp.b
+type plain (pp:plain_package) = p:bytes{pp.valid_length (Seq.length p)}
+abstract type protected_plain (pp:plain_package) (#id:eqtype) (i:id) = plain pp
 
-type plain = bytes
-abstract type protected_plain (pp:plain_package) (#id:eqtype) (i:id) = bytes
-
+val length: (#pp:plain_package) -> (#id:eqtype) -> (#i:id) -> (p:protected_plain pp i) -> n:nat{pp.valid_length n}
 let length (#pp:plain_package) (#id:eqtype) (#i:id) (p:protected_plain pp i) =
-  //length_reveal p;
-  //UInt32.uint_to_t (Seq.length p)
   Seq.length p
 
-val coerce: (#pp:plain_package) -> #key_length:(n:nat{n<=32}) -> (#id:eqtype) -> (#i:id) -> (#key_type:(id -> Type0)) -> (kp:KEY.key_package #id key_length key_type) -> (key:key_type i{KEY.(kp.hon) key == false \/ ~pp.b}) -> p:plain -> p:protected_plain pp i
+val coerce: (#pp:plain_package) -> #key_length:(n:nat{n<=32}) -> (#id:eqtype) -> (#i:id) -> (#key_type:(id -> Type0)) -> (kp:KEY.key_package #id key_length key_type) -> (key:key_type i{KEY.(kp.hon) key == false \/ ~pp.flag}) -> p:plain pp -> p:protected_plain pp i
 let coerce #pp #key_length #id #i #kt kp key p =
   p
 
-val repr: (#pp:plain_package) -> #key_length:(n:nat{n<=32}) -> (#id:eqtype) -> (#i:id) -> (#key_type:(id -> Type0)) -> (kp:KEY.key_package #id key_length key_type) -> (key:key_type i{KEY.(kp.hon) key == false \/ ~pp.b}) -> p:protected_plain pp i -> p:plain
+val repr: (#pp:plain_package) -> #key_length:(n:nat{n<=32}) -> (#id:eqtype) -> (#i:id) -> (#key_type:(id -> Type0)) -> (kp:KEY.key_package #id key_length key_type) -> (key:key_type i{KEY.(kp.hon) key == false \/ ~pp.flag}) -> p:protected_plain pp i -> p:plain pp
 let repr #pp #key_length #id #i #kt kp key p =
   p
